x

src/Mail2/MailServerHAPI.v
@@ -7,77 +7,30 @@ Require Import MailboxAPI.
 Require Import MailboxImpl.
 
 
-Module HLayer (l : Layer) <: Layer.
-
-  Definition opT := horizOpT string l.opT.
-  Definition State := horizState string l.State.
-  Definition step := horizStep string l.step.
-
+Module StringIdx <: HIndex.
+  Definition indexT := string.
   Definition indexValid (u : string) := u = "Alice"%string \/ u = "Bob"%string.
+  Definition indexCmp := string_Ordering.
+End StringIdx.
 
-  Definition initP : State -> Prop :=
-    horizInitP indexValid l.initP.
+Module MailServerHOp := HOps MailServerOp StringIdx.
+Module MailServerHState := HState MailServerState StringIdx.
+Module MailServerHAPI := HLayer MailServerOp MailServerState MailServerAPI StringIdx.
 
-End HLayer.
-
-
-Module MailServerHAPI := HLayer MailServerAPI.
-Module MailServerLockAbsHAPI := HLayer MailServerLockAbsAPI.
-Module MailboxRestrictedHAPI := HLayer MailboxRestrictedAPI.
-
-
-Module MailServerH <: LayerImpl MailServerLockAbsHAPI MailServerHAPI.
-
-  Definition absR := horizAbsR string MailServerLockAbsImpl.absR.
-
-  Definition compile_ts (ts : @threads_state MailServerHAPI.opT) := ts.
-
-  Theorem compile_ts_no_atomics :
-    forall (ts : @threads_state MailServerHAPI.opT),
-      no_atomics_ts ts ->
-      no_atomics_ts (compile_ts ts).
-  Proof.
-    unfold compile_ts; eauto.
-  Qed.
-
-  Theorem absR_ok :
-    op_abs absR MailServerLockAbsHAPI.step MailServerHAPI.step.
-  Proof.
-    eapply horizAbsR_ok.
-    apply MailServerLockAbsImpl.absR_ok.
-  Qed.
-
-  Hint Resolve absR_ok.
-
-  Theorem compile_traces_match :
-    forall ts,
-      no_atomics_ts ts ->
-      traces_match_abs absR MailServerLockAbsHAPI.initP MailServerLockAbsHAPI.step MailServerHAPI.step (compile_ts ts) ts.
-  Proof.
-    unfold compile_ts, traces_match_abs; intros.
-    eexists; intuition idtac.
-    eapply trace_incl_abs; eauto.
-    eauto.
-  Qed.
-
-  Theorem absInitP :
-    forall s1 s2,
-      MailServerLockAbsHAPI.initP s1 ->
-      absR s1 s2 ->
-      MailServerHAPI.initP s2.
-  Proof.
-    eapply horizAbsR_initP_ok.
-    eapply MailServerLockAbsImpl.absInitP.
-  Qed.
-
-End MailServerH.
+Module MailServerLockAbsHState := HState MailServerLockAbsState StringIdx.
+Module MailServerLockAbsHAPI := HLayer MailServerOp MailServerLockAbsState MailServerLockAbsAPI StringIdx.
 
 
-Module MailboxH <: LayerImpl MailServerLockAbsHAPI MailboxRestrictedHAPI.
+Module MailServerLockAbsImplH' :=
+  LayerImplAbsHT
+    MailServerOp
+    MailServerLockAbsState MailServerLockAbsAPI
+    MailServerState MailServerAPI
+    MailServerLockAbsImpl'
+    StringIdx.
 
-  Definition compile_op T (op : MailServerLockAbsHAPI.opT T) : proc MailboxRestrictedHAPI.opT T :=
-    match op with
-    | Slice i op => SliceProc i (AtomicReaderRestricted.compile_op op)
-    end.
-
-  
+Module MailServerLockAbsImplH :=
+  LayerImplAbs MailServerHOp
+    MailServerLockAbsHState MailServerLockAbsHAPI
+    MailServerHState        MailServerHAPI
+    MailServerLockAbsImplH'.
